iris/SpecFileclose.v
@@ -191,7 +191,7 @@ Global Instance fclose_names_inhabited : Inhabited fclose_names :=
     [] 0%nat 1%positive 1%positive (1%positive, 1%positive)
     (UartNames 1%positive 1%positive 1%positive 1%positive)
     (DiskNames 1%positive 1%positive 1%positive 1%positive 1%positive 1%positive
-               1%positive 1%positive)
+               1%positive 1%positive 1%positive)
     1%positive
     (mword_of_int 0) (mword_of_int 0) (mword_of_int 0)
     (MkBioNames 1%positive 1%positive
